More general restrict

theories/stdpp_restrict.v
@@ -1,215 +1,197 @@
 From Coq Require Import ssreflect.
-From stdpp Require Import countable gmap list.
+From stdpp Require Import fin_maps fin_map_dom.
 
-Section restrict_keys.
-  Context {K M D} `{FinMap K M, ElemOf K D, !RelDecision (∈@{D})}.
+Definition restrict {K M} `{FinMap K M}
+  {D} (P: K -> D -> Prop) s `{∀ k, Decision (P k s)}
+  {A} (m: M A) :=
+  filter (fun '(k,_) => P k s) m.
 
-  (** Restrict a map's keys to a given set *)
-  Definition restrict_keys {A} (s:D) (m:M A) := filter (fun '(k,_) => k ∈ s) m.
+Section restrict.
+  Context {K M} `{FinMap K M}.
 
-  Lemma restrict_keys_filter {A} s (m:M A) :
-    restrict_keys s m = filter (fun '(k,_) => k ∈ s) m.
-  Proof. reflexivity. Qed.
+  Section simple_facts.
+    Context {D} (P: K -> D -> Prop) s `{∀ k, Decision (P k s)}.
+    Context {A} (m:M A).
 
-  Lemma restrict_keys_lookup_Some {A} s (m:M A) k v:
-    restrict_keys s m !! k = Some v <-> m !! k = Some v /\ k ∈ s.
-  Proof. apply map_filter_lookup_Some. Qed.
+    (* In case we feel another definition would be better *)
+    Lemma restrict_filter: restrict P s m = filter (fun '(k,_) => P k s) m.
+    Proof. reflexivity. Qed.
 
-  Lemma restrict_keys_lookup_Some_2 {A} s (m:M A) k v:
-    m !! k = Some v -> k ∈ s -> restrict_keys s m !! k = Some v.
-  Proof. intros. rewrite restrict_keys_lookup_Some. done. Qed.
+    Lemma restrict_lookup_Some k v:
+      restrict P s m !! k = Some v <-> m !! k = Some v /\ P k s.
+    Proof. apply map_filter_lookup_Some. Qed.
 
-  Lemma restrict_keys_lookup_None {A} s (m:M A) k:
-    restrict_keys s m !! k = None <-> m !! k = None \/ k ∉ s.
+    Lemma restrict_lookup_Some_2 k v:
+      m !! k = Some v -> P k s -> restrict P s m !! k = Some v.
+    Proof. intros. rewrite restrict_lookup_Some. done. Qed.
+
+    Lemma restrict_lookup_None k:
+      restrict P s m !! k = None <-> m !! k = None \/ ¬ P k s.
+    Proof.
+      split. intros Hr.
+      destruct (m!!k) eqn:Hm.
+        destruct (decide (k ∈ s)) as [Heq|Heq].
+          rewrite (restrict_lookup_Some_2 k _ Hm Heq) in Hr. discriminate.
+          right. done.
+        left. done.
+      destruct (restrict P s m !! k) eqn:Hm; [ | reflexivity ].
+      apply restrict_lookup_Some in Hm as [Hmk Hp].
+      intros [Hmk' | Hp'].
+        rewrite -Hmk. exact Hmk'.
+        contradiction (Hp' Hp).
+    Qed.
+
+    Lemma restrict_lookup_None_2l k:
+      m !! k = None -> restrict P s m !! k = None.
+    Proof. intros. rewrite restrict_lookup_None. left. done. Qed.
+
+    Lemma restrict_lookup_None_2r k:
+      ¬ P k s -> restrict P s m !! k = None.
+    Proof. intros. rewrite restrict_lookup_None. right. done. Qed.
+
+    Lemma restrict_subseteq: restrict P s m ⊆ m.
+    Proof. apply map_filter_subseteq. Qed.
+
+    Lemma dom_restrict_subseteq
+      `{∀ A : Type, Dom (M A) D, ElemOf K D, Empty D, Singleton K D,
+      Union D, Intersection D, Difference D, !FinMapDom K M D}:
+      dom (restrict P s m) ⊆ dom m.
+    Proof. apply subseteq_dom, restrict_subseteq. Qed.
+
+    Lemma restrict_lookup k:
+      restrict P s m !! k = (m !! k) ≫= λ v,
+      match decide (P k s) with
+        |left _ => Some v
+        |right _ => None
+      end.
+    Proof.
+      destruct (m!!k) eqn:Hm.
+      destruct (decide (P k s)) as [Hk|Hk].
+      simpl. rewrite restrict_lookup_Some. done.
+      simpl. apply restrict_lookup_None_2r. done.
+      simpl. apply restrict_lookup_None_2l. done.
+    Qed.
+
+  End simple_facts.
+
+  Lemma restrict_restrict
+    {D1 D2} (P1: K -> D1 -> Prop) (P2: K -> D2 -> Prop) s1 s2
+    `{∀ s1 k, Decision (P1 k s1)} `{∀ s2 k, Decision (P2 k s2)}
+    {A} (m:M A):
+    restrict P1 s1 (restrict P2 s2 m) = restrict (fun k s => P1 k s1 /\ P2 k s2) (s1,s2) m.
+  Proof. apply map_filter_filter. Qed.
+
+  Lemma restrict_restrict_comm
+    {D1 D2} (P1: K -> D1 -> Prop) (P2: K -> D2 -> Prop) s1 s2
+    `{∀ s1 k, Decision (P1 k s1)} `{∀ s2 k, Decision (P2 k s2)}
+    {A} (m:M A):
+    restrict P1 s1 (restrict P2 s2 m) = restrict P2 s2 (restrict P1 s1 m).
   Proof.
-    split. intros Hr.
-    destruct (m!!k) eqn:Hm.
-      destruct (decide (k ∈ s)) as [Heq|Heq].
-        rewrite (restrict_keys_lookup_Some_2 _ m k _ Hm Heq) in Hr. discriminate.
-        right. done.
-      left. done.
-    destruct (restrict_keys s m !! k) eqn:Hm; [ | reflexivity ].
-    apply restrict_keys_lookup_Some in Hm as [Hmk Hp].
-    intros [Hmk' | Hp'].
-      rewrite -Hmk. exact Hmk'.
-      contradiction (Hp' Hp).
+    rewrite !restrict_restrict.
+    apply map_filter_ext. intros. split; intros []; done.
   Qed.
 
-  Lemma restrict_keys_lookup_None_2l {A} s (m:M A) k:
-    m !! k = None -> restrict_keys s m !! k = None.
-  Proof. intros. rewrite restrict_keys_lookup_None. left. done. Qed.
-
-  Lemma restrict_keys_lookup_None_2r {A} s (m:M A) k:
-    k ∉ s -> restrict_keys s m !! k = None.
-  Proof. intros. rewrite restrict_keys_lookup_None. right. done. Qed.
-
-  Lemma restrict_keys_subseteq {A} s (m:M A) :
-    restrict_keys s m ⊆ m.
-  Proof. apply map_filter_subseteq. Qed.
-
-  Lemma restrict_keys_lookup {A} s (m:M A) k :
-    restrict_keys s m !! k = (m !! k) ≫= λ v,
-    match decide (k ∈ s) with
-      |left _ => Some v
-      |right _ => None
-    end.
-  Proof.
-    destruct (m!!k) eqn:Hm.
-    destruct (decide (k ∈ s)) as [Hk|Hk].
-    simpl. rewrite restrict_keys_lookup_Some. done.
-    simpl. apply restrict_keys_lookup_None_2r. done.
-    simpl. apply restrict_keys_lookup_None_2l. done.
-  Qed.
-
-  Lemma restrict_keys_restrict_keys `{Empty D, Singleton K D,
-    Union D, Intersection D, Difference D, !Set_ K D}
-    {A} s s' (m:M A) :
-    restrict_keys s (restrict_keys s' m) = restrict_keys (s ∩ s') m.
-  Proof.
-    unfold restrict_keys.
-    rewrite map_filter_filter -map_filter_ext.
-    intros. rewrite elem_of_intersection. done.
-  Qed.
-
-  Lemma restrict_keys_merge {A B C} s ml mr (f: option A -> option B -> option C) :
-    restrict_keys s (merge f ml mr) =
-    merge f (restrict_keys s ml) (restrict_keys s mr).
+  Lemma restrict_merge
+    {D} (P: K -> D -> Prop) s `{∀ k, Decision (P k s)}
+    {A B C} ml mr (f: option A -> option B -> option C) :
+    restrict P s (merge f ml mr) =
+    merge f (restrict P s ml) (restrict P s mr).
   Proof.
     apply map_eq. intros k.
-    rewrite restrict_keys_lookup !lookup_merge !restrict_keys_lookup.
-    destruct (ml!!k); destruct (mr!!k); destruct (decide (k∈ s)); simpl.
+    rewrite restrict_lookup !lookup_merge !restrict_lookup.
+    destruct (ml!!k); destruct (mr!!k); destruct (decide (P k s)); simpl.
     all: match goal with
     | |- ?x ≫= _ = _ => destruct x; try reflexivity
     | |- _ => reflexivity
     end.
   Qed.
 
-  Lemma restrict_keys_map_zip_with {A B C} s ml mr (f: A -> B -> C) :
-    restrict_keys s (map_zip_with f ml mr) =
-    map_zip_with f (restrict_keys s ml) (restrict_keys s mr).
-  Proof. apply restrict_keys_merge. Qed.
-
-  Lemma dom_restrict_keys_subseteq_l
-    `{∀ A : Type, Dom (M A) D, Empty D, Singleton K D,
-      Union D, Intersection D, Difference D, !FinMapDom K M D}
-    {A} s (m:M A) :
-    dom (restrict_keys s m) ⊆ s.
-  Proof.
-    intros x Hx. apply elem_of_dom in Hx as [y Hx].
-    apply restrict_keys_lookup_Some in Hx as [_ Hx]. exact Hx.
-  Qed.
-
-  Lemma dom_restrict_keys_subseteq_r
-    `{∀ A : Type, Dom (M A) D, Empty D, Singleton K D,
-      Union D, Intersection D, Difference D, !FinMapDom K M D}
-    {A} s (m:M A) :
-    dom (restrict_keys s m) ⊆ dom m.
-  Proof. apply subseteq_dom. apply restrict_keys_subseteq. Qed.
-End restrict_keys.
-
-Section restrict.
-  Context {K M D} `{FinMapDom K M D, !RelDecision (∈@{D})}.
-
-  (** Restrict m to only contain s's keys  *)
-  Definition restrict {A B} (s:M A) (m: M B) := restrict_keys (dom s) m.
-
-  Lemma restrict_lookup_Some {A B} (s:M A) (m: M B) k v :
-    restrict s m !! k = Some v <-> m !! k = Some v /\ is_Some (s !! k).
-  Proof. rewrite restrict_keys_lookup_Some elem_of_dom. done. Qed.
-
-  Lemma restrict_lookup_Some_2 {A B} (s:M A) (m: M B) k v :
-    m !! k = Some v -> is_Some(s !! k) -> restrict s m !! k = Some v.
-  Proof. intros. rewrite restrict_lookup_Some. done. Qed.
-
-  Lemma restrict_lookup_None {A B} (s:M A) (m: M B) k:
-    restrict s m !! k = None <-> m !! k = None \/ s !! k = None.
-  Proof. rewrite restrict_keys_lookup_None not_elem_of_dom. done. Qed.
-
-  Lemma restrict_lookup_None_2l {A B} (s:M A) (m: M B) k:
-    m !! k = None -> restrict s m !! k = None.
-  Proof. intros. rewrite restrict_lookup_None. left. done. Qed.
-
-  Lemma restrict_lookup_None_2r {A B} (s:M A) (m: M B) k:
-    s !! k = None -> restrict s m !! k = None.
-  Proof. intros. rewrite restrict_lookup_None. right. done. Qed.
-
-  Lemma restrict_subseteq {A B} (s:M A) (m: M B) :
-    restrict s m ⊆ m.
-  Proof. apply restrict_keys_subseteq. Qed.
-
-  Lemma dom_restrict {A B} (s:M A) (m: M B) :
-    dom (restrict s m) ≡@{D} dom s ∩ dom m.
-  Proof.
-    rewrite set_equiv. intros k.
-    rewrite elem_of_intersection !elem_of_dom.
-    split.
-    - intros [v Hv]. apply restrict_lookup_Some in Hv as [Hv2 Hv1].
-      apply mk_is_Some in Hv2. done.
-    - intros [Hv1 [v Hv2]]. exists v.
-      rewrite restrict_keys_lookup_Some elem_of_dom.
-      done.
-  Qed.
-
-  Lemma dom_restrict_L `{!LeibnizEquiv D} {A B} (s:M A) (m: M B) :
-    dom (restrict s m) = dom s ∩ dom m.
-  Proof. unfold_leibniz. apply dom_restrict. Qed.
-
-  Lemma restrict_lookup {A B} (s:M A) (m: M B) k:
-    restrict s m !! k = m !! k ≫= λ v, s !! k ≫= λ _, Some v.
-  Proof.
-    rewrite restrict_keys_lookup.
-    destruct (m!!k); simpl. destruct (s!!k) eqn:Hm1;
-    destruct (decide (k ∈ dom s)) as [Heq|Heq].
-    reflexivity.
-    rewrite not_elem_of_dom Hm1 in Heq. discriminate.
-    rewrite elem_of_dom Hm1 in Heq. contradiction (is_Some_None Heq).
-    reflexivity.
-    reflexivity.
-  Qed.
-
-  Global Instance restrict_idemp {A} : IdemP (=@{M A}) restrict.
-  Proof.
-    intros m. apply map_eq. intros k. destruct (m!!k) eqn:Hm.
-    apply (restrict_lookup_Some_2 _ _ _ _ Hm (mk_is_Some _ _ Hm)).
-    apply (restrict_lookup_None_2l _ _ _ Hm).
-  Qed.
-
-  Lemma restrict_merge {A B B' B''} (s:M A) ml mr (f: option B -> option B' -> option B'') :
-    restrict s (merge f ml mr) =
-    merge f (restrict s ml) (restrict s mr).
-  Proof. apply restrict_keys_merge. Qed.
-
-  Lemma restrict_map_zip_with {A B B' B''} (s:M A) ml mr (f: B -> B' -> B'') :
-    restrict s (map_zip_with f ml mr) =
-    map_zip_with f (restrict s ml) (restrict s mr).
+  Lemma restrict_map_zip_with
+    {D} (P: K -> D -> Prop) s `{∀ k, Decision (P k s)}
+    {A B C} ml mr (f: A -> B -> C) :
+    restrict P s (map_zip_with f ml mr) =
+    map_zip_with f (restrict P s ml) (restrict P s mr).
   Proof. apply restrict_merge. Qed.
 
-  Lemma dom_restrict_subseteq_l {A B} (s:M A) (m:M B):
-    dom (restrict s m) ⊆ dom s.
-  Proof.
-    intros x Hx. apply elem_of_dom in Hx as [y Hx].
-    apply restrict_keys_lookup_Some in Hx as [_ Hx]. exact Hx.
-  Qed.
+  (** Common case: restrict keys to elements of a set *)
+  Section restrict_set.
+    Context `{ElemOf K D, !RelDecision (∈@{D})}.
 
-  Lemma dom_restrict_subseteq_r {A B} (s:M A) (m:M B):
-    dom (restrict s m) ⊆ dom m.
-  Proof. apply subseteq_dom. apply restrict_subseteq. Qed.
+    Definition restrict_set (s:D) {A} (m:M A) := restrict (∈) s m.
+
+    Lemma dom_restrict_set_subseteq
+      `{∀ A : Type, Dom (M A) D, Empty D, Singleton K D,
+        Union D, Intersection D, Difference D, !FinMapDom K M D}
+      {A} s (m:M A) :
+      dom (restrict_set s m) ⊆ s.
+    Proof.
+      intros x Hx. apply elem_of_dom in Hx as [y Hx].
+      apply restrict_lookup_Some in Hx as [_ Hx]. exact Hx.
+    Qed.
+
+    Lemma restrict_set_restrict_set `{Empty D, Singleton K D,
+      Union D, Intersection D, Difference D, !Set_ K D}
+      {A} s1 s2 (m:M A) :
+      restrict_set s1 (restrict_set s2 m) = restrict_set (s1 ∩ s2) m.
+    Proof.
+      unfold restrict_set.
+      specialize (restrict_restrict (∈) (∈) s1 s2 m) as Hx. rewrite Hx. clear Hx.
+      rewrite -map_filter_ext. intros. rewrite elem_of_intersection. done.
+    Qed.
+  End restrict_set.
+
+  (** Another common case: restrict to keys present in another map *)
+  Section restrict_map.
+    Definition restrict_map {A B} (s:M A) (m:M B) :=
+      restrict (fun k s => is_Some(s!!k)) s m.
+
+    Global Instance restrict_idemp {A} : IdemP (=@{M A}) restrict_map.
+    Proof.
+      intros m. apply map_eq. intros k. destruct (m!!k) as [v|] eqn:Hm.
+      apply restrict_lookup_Some_2. apply Hm. exists v. apply Hm.
+      apply restrict_lookup_None_2l. apply Hm.
+    Qed.
+
+    Context `{∀ A : Type, Dom (M A) D, ElemOf K D, Empty D, Singleton K D,
+      Union D, Intersection D, Difference D, !FinMapDom K M D, !RelDecision (∈@{D})}.
+
+    Lemma restrict_map_restrict_set {A B} (s:M A) (m:M B):
+      restrict_map s m = restrict_set (dom s) m.
+    Proof. apply map_filter_ext. intros. rewrite elem_of_dom. reflexivity. Qed.
+
+    Lemma dom_restrict_map {A B} (s:M A) (m:M B):
+      dom (restrict_map s m) ≡@{D} dom s ∩ dom m.
+    Proof.
+      rewrite set_equiv. intros k.
+      rewrite elem_of_intersection !elem_of_dom.
+      split.
+      - intros [v Hv]. apply restrict_lookup_Some in Hv as [Hv2 Hv1].
+        apply mk_is_Some in Hv2. done.
+      - intros [Hv1 [v Hv2]]. exists v.
+        rewrite restrict_lookup_Some. done.
+    Qed.
+
+    Lemma dom_restrict_L `{!LeibnizEquiv D} {A B} (s:M A) (m: M B) :
+      dom (restrict_map s m) = dom s ∩ dom m.
+    Proof. unfold_leibniz. apply dom_restrict_map. Qed.
+
+    Lemma dom_restrict_map_subseteq {A B} (s:M A) (m:M B):
+      dom (restrict_map s m) ⊆ dom s.
+    Proof.
+      intros x Hx. apply elem_of_dom in Hx as [y Hx].
+      apply restrict_lookup_Some in Hx as [_ Hx]. apply elem_of_dom. exact Hx.
+    Qed.
+  End restrict_map.
 End restrict.
 
 
 (** map_zip ignores keys that aren't shared by both maps *)
 Lemma map_zip_minimal {K M A B} `{FinMapDom K M D, !RelDecision (∈@{D})} (m1: M A) (m2: M B) :
   map_zip m1 m2 =
-  map_zip (restrict m2 m1) (restrict m1 m2).
+  map_zip (restrict_map m2 m1) (restrict_map m1 m2).
 Proof.
   apply map_eq. intros k.
-  rewrite !map_lookup_zip_with.
+  rewrite !map_lookup_zip_with !restrict_lookup.
   destruct (m1 !! k) as [v1|] eqn:Hm1;
-  destruct (m2 !! k) as [v2|] eqn:Hm2; simpl.
-  - rewrite (restrict_lookup_Some_2 _ _ _ _ Hm2 (mk_is_Some _ _ Hm1)).
-    rewrite (restrict_lookup_Some_2 _ _ _ _ Hm1 (mk_is_Some _ _ Hm2)).
-    reflexivity.
-  - rewrite (restrict_lookup_None_2r _ _ _ Hm2). reflexivity.
-  - rewrite (restrict_lookup_None_2l _ _ _ Hm1). reflexivity.
-  - rewrite (restrict_lookup_None_2r _ _ _ Hm2). reflexivity.
+  destruct (m2 !! k) as [v2|] eqn:Hm2; reflexivity.
 Qed.
